0 (#229)
This PR solves problem 0.

HumanEvalLean/HumanEval0.lean
@@ -1,5 +1,334 @@
-def has_close_elements : Unit :=
-  ()
+import Std
+open Std Std.Do
+
+set_option mvcgen.warning false
+
+/-!
+## Missing API
+-/
+
+@[simp, grind =]
+theorem Subarray.size_drop {xs : Subarray α} {n : Nat} :
+    (xs.drop n).size = xs.size - n := by
+  simp only [size, stop, drop, start]
+  omega
+
+@[grind =, simp]
+theorem Subarray.size_mkSlice_rio {xs : Subarray α} :
+    xs[*...i].size = min i xs.size := by
+  simp [← Subarray.size_toArray]
+
+@[grind =, simp]
+theorem Subarray.size_mkSlice_rci {xs : Subarray α} :
+    xs[i...*].size = xs.size - i := by
+  simp [← Subarray.size_toArray]
+
+namespace Array
+
+def MergeSort.merge (xs ys : Array α) (le : α → α → Bool := by exact (· ≤ ·)) : Array α :=
+  if hxs : 0 < xs.size then
+    if hys : 0 < ys.size then
+      go xs[*...*] ys[*...*] (by simp only [Array.size_mkSlice_rii]; omega) (by simp only [Array.size_mkSlice_rii]; omega) (Array.emptyWithCapacity (xs.size + ys.size))
+    else
+      xs
+  else
+    ys
+where
+  go (xs ys : Subarray α) (hxs : 0 < xs.size) (hys : 0 < ys.size) (acc : Array α) : Array α :=
+    let x := xs[0]
+    let y := ys[0]
+    if le x y then
+      if hi : 1 < xs.size then
+        go (xs.drop 1) ys (by simp only [Subarray.size_drop]; omega) hys (acc.push x)
+      else
+        ys.foldl (init := acc.push x) (fun acc y => acc.push y)
+    else
+      if hj : 1 < ys.size then
+        go xs (ys.drop 1) hxs (by simp only [Subarray.size_drop]; omega) (acc.push y)
+      else
+        xs.foldl (init := acc.push y) (fun acc x => acc.push x)
+  termination_by xs.size + ys.size
+
+def _root_.Subarray.mergeSort (xs : Subarray α) (le : α → α → Bool := by exact (· ≤ ·)) : Array α :=
+    if h : 1 < xs.size then
+      let splitIdx := (xs.size + 1) / 2 -- We follow the same splitting convention as `List.mergeSort`
+      let left := xs[*...splitIdx]
+      let right := xs[splitIdx...*]
+      MergeSort.merge (mergeSort left le) (mergeSort right le) le
+    else
+      xs
+termination_by xs.size
+decreasing_by
+  · simp only [Subarray.size_mkSlice_rio]; omega
+  · simp only [Subarray.size_mkSlice_rci]; omega
+
+def mergeSort (xs : Array α) (le : α → α → Bool := by exact (· ≤ ·)) : Array α :=
+    xs[*...*].mergeSort le
+
+end Array
+
+theorem Subarray.sliceSize_eq_size {xs : Subarray α} :
+    Std.Slice.size xs = xs.size := by
+  rfl
+
+theorem Subarray.getElem_eq_getElem_array {xs : Subarray α} {h : i < xs.size} :
+    xs[i] = xs.array[xs.start + i]'(by simp only [size] at h; have := xs.stop_le_array_size; omega) := by
+  rfl
+
+-- The current `List.extract_eq_drop_take` should be called `List.extract_eq_take_drop`
+@[simp] theorem List.extract_eq_drop_take' {l : List α} {start stop : Nat} :
+    l.extract start stop = (l.take stop).drop start := by
+  simp [List.take_drop]
+  by_cases start ≤ stop
+  · simp [*]
+  · have h₁ : stop - start = 0 := by omega
+    have h₂ : min stop l.length ≤ stop := by omega
+    simp only [Nat.add_zero, drop_take_self, nil_eq, drop_eq_nil_iff, length_take, ge_iff_le, h₁]
+    omega
+
+theorem Subarray.toList_eq_drop_take {xs : Subarray α} :
+    xs.toList = (xs.array.toList.take xs.stop).drop xs.start := by
+  rw [Subarray.toList_eq, Array.toList_extract, List.extract_eq_drop_take']
+
+theorem Subarray.getElem_toList {xs : Subarray α} {h : i < xs.toList.length} :
+    xs.toList[i]'h = xs[i]'(by simpa using h) := by
+  simp [getElem_eq_getElem_array, toList_eq_drop_take]
+
+theorem Subarray.getElem_eq_getElem_toList {xs : Subarray α} {h : i < xs.size} :
+    xs[i]'h = xs.toList[i]'(by simpa using h) := by
+  rw [getElem_toList]
+
+theorem Std.Slice.fold_iter [ToIterator (Slice γ) Id α β]
+    [Iterator α Id β] [IteratorLoop α Id Id] [Iterators.Finite α Id] {s : Slice γ} :
+    s.iter.fold (init := init) f = s.foldl (init := init) f := by
+  rfl
+
+theorem Std.Slice.foldl_toList [ToIterator (Slice γ) Id α β]
+    [Iterator α Id β] [IteratorLoop α Id Id] [LawfulIteratorLoop α Id Id]
+    [Iterators.Finite α Id] {s : Slice γ} :
+    s.toList.foldl (init := init) f = s.foldl (init := init) f := by
+  simp [← Std.Slice.toList_iter, Iter.foldl_toList, fold_iter]
+
+theorem Subarray.fold_iter {xs : Subarray α} :
+    xs.iter.fold (init := init) f = xs.foldl (init := init) f := by
+  rfl
+
+theorem Subarray.foldl_toList {xs : Subarray α} :
+    xs.toList.foldl (init := init) f = xs.foldl (init := init) f := by
+  simp only [← Std.Slice.toList_iter, Iter.foldl_toList, fold_iter]
+
+theorem Subarray.toList_drop {xs : Subarray α} :
+    (xs.drop n).toList = xs.toList.drop n := by
+  simp [Subarray.toList_eq_drop_take, drop, start, stop, array]
+
+theorem Array.MergeSort.merge.go_eq_listMerge {xs ys : Subarray α} {hxs hys le acc} :
+    (Array.MergeSort.merge.go le xs ys hxs hys acc).toList = acc.toList ++ List.merge xs.toList ys.toList le := by
+  fun_induction Array.MergeSort.merge.go le xs ys hxs hys acc
+  · rename_i xs ys _ _ _ _ _ _ _ _
+    rw [List.merge.eq_def]
+    split
+    · have : xs.size = 0 := by simp [← Subarray.length_toList, *]
+      omega
+    · have : ys.size = 0 := by simp [← Subarray.length_toList, *]
+      omega
+    · rename_i x' xs' y' ys' _ _
+      simp +zetaDelta only at *
+      have h₁ : x' = xs[0] := by simp [Subarray.getElem_eq_getElem_toList, *]
+      have h₂ : y' = ys[0] := by simp [Subarray.getElem_eq_getElem_toList, *]
+      cases h₁
+      cases h₂
+      simp [Subarray.toList_drop, *]
+  · rename_i xs ys _ _ _ _ _ _ _
+    rw [List.merge.eq_def]
+    split
+    · have : xs.size = 0 := by simp [← Subarray.length_toList, *]
+      omega
+    · have : ys.size = 0 := by simp [← Subarray.length_toList, *]
+      omega
+    · rename_i x' xs' y' ys' _ _
+      simp +zetaDelta only at *
+      have h₁ : x' = xs[0] := by simp [Subarray.getElem_eq_getElem_toList, *]
+      have h₂ : y' = ys[0] := by simp [Subarray.getElem_eq_getElem_toList, *]
+      cases h₁
+      cases h₂
+      simp [*]
+      have : xs.size = xs'.length + 1 := by simp [← Subarray.length_toList, *]
+      have : xs' = [] := List.eq_nil_of_length_eq_zero (by omega)
+      simp [this]
+      rw [← Subarray.foldl_toList]
+      simp [*]
+  · rename_i xs ys _ _ _ _ _ _ _ _
+    rw [List.merge.eq_def]
+    split
+    · have : xs.size = 0 := by simp [← Subarray.length_toList, *]
+      omega
+    · have : ys.size = 0 := by simp [← Subarray.length_toList, *]
+      omega
+    · rename_i x' xs' y' ys' _ _
+      simp +zetaDelta only at *
+      have h₁ : x' = xs[0] := by simp [Subarray.getElem_eq_getElem_toList, *]
+      have h₂ : y' = ys[0] := by simp [Subarray.getElem_eq_getElem_toList, *]
+      cases h₁
+      cases h₂
+      simp [Subarray.toList_drop, *]
+  · rename_i xs ys _ _ _ _ _ _ _
+    rw [List.merge.eq_def]
+    split
+    · have : xs.size = 0 := by simp [← Subarray.length_toList, *]
+      omega
+    · have : ys.size = 0 := by simp [← Subarray.length_toList, *]
+      omega
+    · rename_i x' xs' y' ys' _ _
+      simp +zetaDelta only at *
+      have h₁ : x' = xs[0] := by simp [Subarray.getElem_eq_getElem_toList, *]
+      have h₂ : y' = ys[0] := by simp [Subarray.getElem_eq_getElem_toList, *]
+      cases h₁
+      cases h₂
+      simp [*]
+      have : ys.size = ys'.length + 1 := by simp [← Subarray.length_toList, *]
+      have : ys' = [] := List.eq_nil_of_length_eq_zero (by omega)
+      simp [this]
+      rw [← Subarray.foldl_toList]
+      simp [*]
+
+attribute [- simp] List.mkSlice_rio_eq_mkSlice_rco
+  Array.mkSlice_rci_eq_mkSlice_rco
+  Subarray.mkSlice_rio_eq_mkSlice_rco Subarray.mkSlice_rci_eq_mkSlice_rco
+
+theorem Array.MergeSort.merge_eq_listMerge {xs ys : Array α} {le} :
+    (Array.MergeSort.merge xs ys le).toList = List.merge xs.toList ys.toList le := by
+  rw [Array.MergeSort.merge]
+  split <;> rename_i heq₁
+  · split <;> rename_i heq₂
+    · simp [Array.MergeSort.merge.go_eq_listMerge]
+    · have : ys.toList = [] := by simp_all
+      simp [this]
+  · have : xs.toList = [] := by simp_all
+    simp [this]
+
+theorem List.mergeSort_eq_merge_mkSlice {xs : List α} :
+    xs.mergeSort le =
+      if 1 < xs.length then
+        merge (xs[*...((xs.length + 1) / 2)].toList.mergeSort le) (xs[((xs.length + 1) / 2)...*].toList.mergeSort le) le
+      else
+        xs := by
+  fun_cases xs.mergeSort le
+  · simp
+  · simp
+  · rename_i x y ys lr hl hr
+    simp [lr]
+
+theorem Subarray.toList_mergeSort {xs : Subarray α} {le : α → α → Bool} :
+    (xs.mergeSort le).toList = xs.toList.mergeSort le := by
+  fun_induction xs.mergeSort le
+  · rw [List.mergeSort_eq_merge_mkSlice]
+    simp +zetaDelta [Array.MergeSort.merge_eq_listMerge, Subarray.sliceSize_eq_size, *]
+  · simp [List.mergeSort_eq_merge_mkSlice, Subarray.sliceSize_eq_size, *]
+
+theorem Array.toList_mergeSort {xs : Array α} {le : α → α → Bool} :
+    (xs.mergeSort le).toList = xs.toList.mergeSort le := by
+  rw [Array.mergeSort, Subarray.toList_mergeSort, Array.toList_mkSlice_rii]
+
+def Rat.abs (x : Rat) : Rat :=
+  if 0 ≤ x then x else - x
+
+theorem Rat.abs_nonneg {x : Rat} :
+    0 ≤ x.abs := by
+  simp only [Rat.abs]
+  grind
+
+theorem Rat.abs_of_nonneg {x : Rat} (h : 0 ≤ x) :
+    x.abs = x := by
+  grind [Rat.abs]
+
+theorem Rat.abs_sub_comm {x y : Rat} :
+    (x - y).abs = (y - x).abs := by
+  grind [Rat.abs]
+
+theorem Nat.eq_add_of_toList_rio_eq_append_cons {a : Nat} {pref cur suff}
+    (h : (*...a).toList = pref ++ cur :: suff) :
+    cur = pref.length := by
+  have := Rio.eq_succMany?_of_toList_eq_append_cons h
+  simpa [PRange.UpwardEnumerable.least, PRange.least?] using this
+
+@[simp, grind =]
+theorem Array.size_mergeSort {xs : Array α} :
+    (xs.mergeSort le).size = xs.size := by
+  rw [← length_toList, Array.toList_mergeSort, List.length_mergeSort, length_toList]
+
+theorem Array.mergeSort_perm {xs : Array α} :
+    (xs.mergeSort le).Perm xs := by
+  simpa only [perm_iff_toList_perm, Array.toList_mergeSort] using List.mergeSort_perm _ _
+
+theorem Array.Perm.pairwise_iff {R : α → α → Prop} (S : ∀ {x y}, R x y → R y x) :
+    ∀ {l₁ l₂ : Array α} (_p : l₁.Perm l₂), l₁.toList.Pairwise R ↔ l₂.toList.Pairwise R := by
+  intro xs ys
+  simpa only [perm_iff_toList_perm] using List.Perm.pairwise_iff S
+
+theorem Array.pairwise_mergeSort
+    (trans : ∀ (a b c : α), le a b → le b c → le a c)
+    (total : ∀ (a b : α), le a b || le b a) :
+    (l : Array α) → (mergeSort l le).toList.Pairwise (le · ·) := by
+  intro xs
+  simpa [toList_mergeSort] using List.pairwise_mergeSort trans total _
+
+attribute [simp, grind =] Rio.mem_iff
+
+/-!
+## Implementation
+-/
+
+def hasCloseElements (xs : Array Rat) (threshold : Rat) : Bool := Id.run do
+  let sorted := xs.mergeSort
+  for h : i in *...(sorted.size - 1) do
+    if (sorted[i + 1] - sorted[i]).abs < threshold then
+      return true
+  return false
+
+/-!
+## Tests
+-/
+
+example : hasCloseElements #[1.0, 2.0, 3.9, 4.0, 5.0, 2.2] 0.3 = true := by native_decide
+example : hasCloseElements #[1.0, 2.0, 3.9, 4.0, 5.0, 2.2] 0.05 = false := by native_decide
+example : hasCloseElements #[1.0, 2.0, 5.9, 4.0, 5.0] 0.95 = true := by native_decide
+example : hasCloseElements #[1.0, 2.0, 5.9, 4.0, 5.0] 0.8 = false := by native_decide
+example : hasCloseElements #[1.0, 2.0, 3.0, 4.0, 5.0, 2.0] 0.1 = true := by native_decide
+example : hasCloseElements #[1.1, 2.2, 3.1, 4.1, 5.1] 1.0 = true := by native_decide
+example : hasCloseElements #[1.1, 2.2, 3.1, 4.1, 5.1] 0.5 = false := by native_decide
+
+/-!
+## Verification
+-/
+
+theorem hasCloseElements_iff_mergeSort {xs threshold} :
+    hasCloseElements xs threshold ↔ ∃ (i : Nat) (_ : i < xs.mergeSort.size - 1), (xs.mergeSort[i + 1] - xs.mergeSort[i]).abs < threshold := by
+  generalize hwp : hasCloseElements xs threshold = wp
+  apply Id.of_wp_run_eq hwp
+  mvcgen
+  invariants
+  · .withEarlyReturn
+      (fun cur _ => ⌜∀ i < cur.prefix.length, threshold ≤ (xs.mergeSort[i + 1]! - xs.mergeSort[i]!).abs⌝)
+      (fun r _ => ⌜r = true ∧ ∃ (i : Nat) (_ : i < xs.mergeSort.size - 1), (xs.mergeSort[i + 1] - xs.mergeSort[i]).abs < threshold⌝)
+  with grind [Nat.eq_add_of_toList_rio_eq_append_cons, Rio.length_toList, Nat.size_rio]
+
+theorem hasCloseElements_iff {xs threshold} :
+    hasCloseElements xs threshold ↔ ¬ xs.toList.Pairwise (fun a b => threshold ≤ (b - a).abs) := by
+  simp only [hasCloseElements_iff_mergeSort]
+  have := xs.mergeSort_perm (le := (· ≤ ·))
+  rw [← this.pairwise_iff]
+  · apply Iff.intro
+    · simp only [List.pairwise_iff_getElem, Classical.not_forall]
+      grind
+    · simp only [List.pairwise_iff_getElem, Classical.not_forall]
+      rintro ⟨i, j, hi, hj, hij, h⟩
+      refine ⟨i, by grind, ?_⟩
+      have h_sorted := xs.pairwise_mergeSort (le := (· ≤ ·)) (by grind) (by grind)
+      rw [List.pairwise_iff_getElem] at h_sorted
+      rw [Rat.abs_of_nonneg (by grind)] at ⊢ h
+      have : xs.mergeSort[i + 1]'(by grind) ≤ xs.mergeSort[j] := by by_cases i + 1 = j <;> grind
+      grind
+  · simp [Rat.abs_sub_comm]
 
 /-!
 ## Prompt
